RAC of memory properties: semantics of expressions completed + Lemma 5.6

Memory/Semantics.v
@@ -52,14 +52,50 @@ Module Semantics(V : DecidableType)(B: Eqb.EQB)
       check_type Γ (EBinop Oadd e1 e2 (TPtr τ1)) = Ok (TPtr τ1).
   Proof. check_type. Qed.
 
+  Definition within_bounds (κ: mtyp)(n:Z) : option value :=
+    if ((min_int (sizeof κ) <=? n)%Z && (n <=? max_int (sizeof κ))%Z)%bool
+      then ⎣Int n⎦
+    else ⎣Undef⎦.
+
+
+  Definition sem_unop (κ: mtyp) op (v: value) : option value :=
+    match (op,v) with
+    | (_, Undef) => ⎣Undef⎦
+    | (Oneg, Int n) => within_bounds κ (-n)%Z
+    | (Onot, Int n) => ⎣Int(Z.b2z(n =? 0)%Z)⎦
+    | (_, _) => ϵ
+    end.
+                                      
+  Definition sem_binop (κ: mtyp) op (v1 v2: value) : option value :=
+    match (op, v1, v2) with
+    | (Odiv, _, Int 0%Z) => ϵ
+    | (Omod, _, Int 0%Z) => ϵ
+    | (_, Undef, _) => ⎣Undef⎦
+    | (_, _, Undef) => ⎣Undef⎦
+    | (Oadd, Int n1, Int n2) => within_bounds κ (n1 + n2)%Z
+    | (Osub, Int n1, Int n2) => within_bounds κ (n1 - n2)%Z
+    | (Omul, Int n1, Int n2) => within_bounds κ (n1 * n2)%Z
+    | (Odiv, Int n1, Int n2) => within_bounds κ (n1 / n2)%Z
+    | (Omod, Int n1, Int n2) => within_bounds κ (n1 mod n2)%Z
+    | (Oeq, Int n1, Int n2) => ⎣Int(Z.b2z(n1 =? n2)%Z)⎦
+    | (Olt, Int n1, Int n2) => ⎣Int(Z.b2z(n1 <? n2)%Z)⎦
+    | (Ogt, Int n1, Int n2) => ⎣Int(Z.b2z(n1 >? n2)%Z)⎦
+    | (Ole, Int n1, Int n2) => ⎣Int(Z.b2z(n1 <=? n2)%Z)⎦
+    | (Oge, Int n1, Int n2) => ⎣Int(Z.b2z(n1 >=? n2)%Z)⎦
+    | (Oeq, Ptr (b,δ), Ptr(b',δ')) => ⎣Int(Z.b2z( (B.eqb b b') && (Z.eqb δ δ'))%bool)⎦
+    | (_, _, _) => ϵ
+    end.
+
   Inductive eeval: Ctx.context -> Stx.type_env -> Stx.expr -> value -> Prop :=
   | E_int: forall C Γ n τ,
       valid_expr Γ (EInt n τ) ->
       eeval C Γ (EInt n τ) (Int n)
+
   | E_addr: forall C Γ e τ b δ,
       valid_expr Γ e ->
       lveval C Γ e (b,δ) ->
       eeval C Γ (EAddrof e τ) (Ptr(b,δ))
+
   | E_lval: forall C Γ e τ b δ v,
       check_type Γ e = Ok τ -> 
       lveval C Γ e (b,δ) ->
@@ -67,6 +103,20 @@ Module Semantics(V : DecidableType)(B: Eqb.EQB)
       v <> Undef ->
       kind_t τ = kind_v v ->
       eeval C Γ e v
+            
+  | E_unop: forall C Γ op e τ v v',
+      check_type Γ (EUnop op e τ) = Ok τ ->
+      eeval C Γ e v ->
+      sem_unop (mtype τ) op v = ⎣v'⎦ ->
+      eeval C Γ (EUnop op e τ) v'
+
+  | E_binop: forall C Γ op e1 e2 τ v1 v2 v,
+      check_type Γ (EBinop op e1 e2 τ) = Ok τ ->
+      eeval C Γ e1 v1 ->
+      eeval C Γ e2 v2 ->
+      sem_binop (mtype τ) op v1 v2 = ⎣v⎦ ->
+      eeval C Γ (EBinop op e1 e2 τ) v
+         
   | E_parith: forall C Γ e1 τ1 v1 e2 κ2 b δ n sz e v,
       check_type Γ e1 = Ok (TPtr τ1) ->
       check_type Γ e2 = Ok (TInt κ2) ->
@@ -77,9 +127,11 @@ Module Semantics(V : DecidableType)(B: Eqb.EQB)
       e = EBinop Oadd e1 e2 (TPtr τ1) ->
       v = Ptr(b,(δ+n*sz)%Z) ->
       eeval C Γ e v
+
   with lveval: Ctx.context -> Stx.type_env -> Stx.expr -> B.t * Z -> Prop :=
   | LV_var: forall C Γ x τ b,
       lveval C Γ (EVar x τ) (b,0%Z)
+
   | LV_deref: forall C Γ e τ b δ,
       check_type Γ e = Ok (TPtr τ) ->
       eeval C Γ e (Ptr(b,δ)) ->
@@ -103,6 +155,54 @@ Module Semantics(V : DecidableType)(B: Eqb.EQB)
     forall σ Hσ v, kind_v v = kind_v (induced σ Hσ v).
   Proof.
     intros σ Hσ [n|[b δ]|]; trivial.
+  Qed.
+
+  Ltac within_bounds :=
+    let Hcond := fresh "Hcond" in 
+    unfold within_bounds in *;
+    match goal with
+    | [ H: context [ if ?cond then _ else _ ] |- context[if ?cond then _ else _]] =>
+        case_eq(cond); intro Hcond; rewrite Hcond in H;
+        injection H; clear H; intro H; subst; trivial
+    end.
+  
+  Lemma induced_unop:
+    forall τ op σ Hσ v v',
+      sem_unop (mtype τ) op v = ⎣ v' ⎦ ->
+      sem_unop (mtype τ) op (induced σ Hσ v) = ⎣ induced σ Hσ v' ⎦.
+  Proof.
+    unfold sem_unop.
+    intros τ op σ Hσ [n|[b δ]|] v' H; destruct op; simpl in H; simpl;
+      try discriminate;
+      try within_bounds;
+      injection H; clear H; intro H; subst; trivial.
+  Qed.
+
+  Lemma induced_binop:
+    forall κ op σ Hσ v1 v2 v,
+      sem_binop κ op v1 v2 = ⎣ v ⎦ -> 
+      sem_binop κ op (induced σ Hσ v1) (induced σ Hσ v2) = ⎣ induced σ Hσ v ⎦.
+  Proof.
+    intros κ op σ Hσ [n1|[b1 δ1]|][n2|[b2 δ2]|] v H;
+    unfold sem_binop in *; simpl in *;
+      destruct op; simpl in *;
+      try discriminate;
+      try within_bounds;
+      try solve [destruct n2; try discriminate; try within_bounds;
+                 inversion H; now subst];
+      try solve [injection H; clear H; intro H; subst; trivial].
+    assert(Heqb: B.eqb b1 b2 = B.eqb (σ b1) (σ b2)).
+    {
+      case_eq(B.eqb b1 b2); intro HH.
+      - now repeat simpl_block_eqb.
+      - apply Block.eqb_neq in HH.
+        symmetry. apply Bool.not_true_iff_false.
+        contradict HH.
+        simpl_block_eqb.
+        eapply σ_eq; eauto.
+    }
+    rewrite <- Heqb.
+    injection H; clear H; intro H; now subst.
   Qed.
   
   Lemma isomorphic_evalexpr:
@@ -131,8 +231,13 @@ Module Semantics(V : DecidableType)(B: Eqb.EQB)
       eapply E_lval; eauto.
       + now apply induced_undef.
       + now rewrite <- induced_kind.
-    - simpl in *.
-      intros σ Hσ C' Hiso.
+    - simpl in *. intros σ Hσ C' Hiso.
+      eapply E_unop; eauto.
+      now apply induced_unop.
+    - simpl in *. intros σ Hσ C' Hiso.
+      eapply E_binop; eauto.
+      now apply induced_binop.
+    - simpl in *. intros σ Hσ C' Hiso.
       specialize (IHHeeval1 σ Hσ C' Hiso).
       specialize (IHHeeval2 σ Hσ C' Hiso).
       eapply E_parith; eauto.
